proof_irrel.v
@@ -9,24 +9,20 @@ Instance: ProofIrrel True.
 Proof. by intros [] []. Qed.
 Instance: ProofIrrel False.
 Proof. by intros []. Qed.
-
 Instance and_pi (A B : Prop) :
   ProofIrrel A → ProofIrrel B → ProofIrrel (A ∧ B).
 Proof. intros ?? [??] [??]. by f_equal. Qed.
 Instance prod_pi (A B : Type) :
   ProofIrrel A → ProofIrrel B → ProofIrrel (A * B).
 Proof. intros ?? [??] [??]. by f_equal. Qed.
-
 Instance eq_pi {A} `{∀ x y : A, Decision (x = y)} (x y : A) :
   ProofIrrel (x = y).
 Proof.
   intros ??. apply eq_proofs_unicity.
   intros x' y'. destruct (decide (x' = y')); tauto.
 Qed.
-
 Instance Is_true_pi (b : bool) : ProofIrrel (Is_true b).
 Proof. destruct b; simpl; apply _. Qed.
-
 Lemma sig_eq_pi `(P : A → Prop) `{∀ x, ProofIrrel (P x)}
   (x y : sig P) : x = y ↔ `x = `y.
 Proof.
@@ -34,7 +30,6 @@ Proof.
   destruct x as [x Hx], y as [y Hy]; simpl; intros; subst.
   f_equal. apply proof_irrel.
 Qed.
-
 Lemma exists_proj1_pi `(P : A → Prop) `{∀ x, ProofIrrel (P x)}
   (x : sig P) p : `x ↾ p = x.
 Proof. by apply (sig_eq_pi _). Qed.
